compiler/parsing/fromSexpScript.sml
@@ -660,7 +660,6 @@ val sexpop_def = Define`
   if s = "Opw64Add" then SOME (Opw W64 Add) else
   if s = "Opw64Sub" then SOME (Opw W64 Sub) else
   if s = "Equality" then SOME Equality else
-  (* if s = "FPpredFPNaN" then SOME (FP_pred FP_NaN) else *)
   if s = "FPcmpFPLess" then SOME (FP_cmp FP_Less) else
   if s = "FPcmpFPLessEqual" then SOME (FP_cmp FP_LessEqual) else
   if s = "FPcmpFPGreater" then SOME (FP_cmp FP_Greater) else
@@ -1307,7 +1306,6 @@ val opsexp_def = Define`
   (opsexp (Shift W64 Asr n) = SX_CONS (SX_SYM "Shift64Asr") (SX_NUM n)) ∧
   (opsexp (Shift W64 Ror n) = SX_CONS (SX_SYM "Shift64Ror") (SX_NUM n)) ∧
   (opsexp Equality = SX_SYM "Equality") ∧
-  (* (opsexp (FP_pred FP_NaN) = SX_SYM "FPpredFPNaN") /\ *)
   (opsexp (FP_cmp FP_Less) = SX_SYM "FPcmpFPLess") ∧
   (opsexp (FP_cmp FP_LessEqual) = SX_SYM "FPcmpFPLessEqual") ∧
   (opsexp (FP_cmp FP_Greater) = SX_SYM "FPcmpFPGreater") ∧
@@ -1387,7 +1385,7 @@ Proof
   Cases_on`op`>>rw[sexpop_def,opsexp_def]>>
   TRY(MAP_FIRST rename1 [
         ‘Opn c1’, ‘Opb c1’, ‘Opw c2 c1’, ‘Chopb c1’, ‘Shift c1 c2 _’,
-        (*‘FP_pred c1’,*) ‘FP_cmp c1’, ‘FP_uop c1’, ‘FP_bop c1’, `FP_top c1`,
+        ‘FP_cmp c1’, ‘FP_uop c1’, ‘FP_bop c1’, ‘FP_top c1’,
         ‘WordFromInt c1’, ‘WordToInt c1’,
         ‘Real_cmp c1’, ‘Real_bop c1’, ‘Real_uop c1’
       ] >>
