icing/icing_realIdProofsScript.sml
@@ -158,14 +158,15 @@ Proof
     ntac 2 (TOP_CASE_TAC>>simp[])>>
     TOP_CASE_TAC>>fs[]
     >- (
-      fs[astTheory.getOpClass_def]>>
+      fs[]>>
       every_case_tac>>fs[]>>
       fs[isPureOp_def])
     >- (
-      fs[astTheory.getOpClass_def]>>
+      fs[]>>
       every_case_tac>>fs[]>>
       fs[isPureOp_def])
-    >> every_case_tac>>simp[state_component_equality,fpState_component_equality])
+    >> every_case_tac
+    >>gs[state_component_equality,fpState_component_equality, isPureOp_def])
   >- (
     qpat_x_assum` _ = (_,_)` mp_tac>>
     ntac 2 (TOP_CASE_TAC>>simp[])>>
@@ -178,8 +179,8 @@ Proof
       fs[astTheory.getOpClass_def]>>
       every_case_tac>>fs[]>>
       fs[isPureOp_def])
-    >- (every_case_tac>>simp[state_component_equality,fpState_component_equality])
-    >- (every_case_tac>>simp[state_component_equality,fpState_component_equality]))
+    >> every_case_tac
+    >> gs[state_component_equality,fpState_component_equality, isPureOp_def])
   >- (
     qpat_x_assum` _ = (_,_)` mp_tac>>
     ntac 2 (TOP_CASE_TAC>>simp[])>>
