translator/monadic/ml_monadStoreScript.sml
@@ -16,9 +16,6 @@ val SEP_EXISTS_SEPARATE = save_thm("SEP_EXISTS_SEPARATE",
 val SEP_EXISTS_INWARD = save_thm("SEP_EXISTS_INWARD",
   List.nth(SPEC_ALL SEP_CLAUSES |> CONJUNCTS, 1) |> GSYM |> GEN_ALL);
 
-(* Required to finish proofs with evaluate *)
-val _ = augment_srw_ss [rewrites [astTheory.getOpClass_def]];
-
 Theorem ALLOCATE_ARRAY_evaluate:
    !env s n xname xv.
     (nsLookup env.v (Short xname) = SOME xv) ==>
