icing/examples/output/readmePrefix
@@ -1,1 +1,0 @@
-output directory for sexp files
